src/SchedSim.v
@@ -14,17 +14,7 @@ From Fairness Require Import
   FIFOSched.
 From ExtLib Require Import FMapAList.
 
-Tactic Notation "repl" constr(e) "with" constr(e') "at" ne_integer_list(n) :=
-  let x := fresh in
-  set e as x at n;
-  replace x with e';
-  subst x.
-
-Tactic Notation "repl" constr(e) "with" constr(e') "at" ne_integer_list(n) "by" tactic(tac) :=
-  let x := fresh in
-  set e as x at n;
-  replace x with e' by tac;
-  subst x.
+Set Implicit Arguments.
 
 Ltac destruct_itree itr :=
   let E := fresh "E" in
@@ -34,6 +24,201 @@ Ltac destruct_itree itr :=
   apply bisim_is_eq in E;
   subst itr.
 
+Section SSIM.
+
+  Variable wf_src : WF.
+  Variable wf_tgt : WF.
+
+  Inductive _ssim
+    (ssim : forall RT R0 R1 (RR : R0 -> R1 -> Prop), bool -> (@imap thread_id wf_src) -> bool -> (@imap thread_id wf_tgt) -> scheduler RT R0 -> scheduler RT R1 -> Prop)
+    {RT R0 R1} (RR : R0 -> R1 -> Prop)
+    (p_src : bool) (m_src : @imap thread_id wf_src) (p_tgt : bool) (m_tgt : @imap thread_id wf_tgt)
+    : scheduler RT R0 -> scheduler RT R1 -> Prop :=
+
+  | ssim_ret
+      r_src r_tgt
+      (SIM : RR r_src r_tgt)
+    : _ssim ssim RR p_src m_src p_tgt m_tgt (Ret r_src) (Ret r_tgt)
+
+  | ssim_tauL
+      itr_src itr_tgt
+      (SIM : _ssim ssim RR true m_src p_tgt m_tgt itr_src itr_tgt)
+    : _ssim ssim RR p_src m_src p_tgt m_tgt (Tau itr_src) itr_tgt
+
+  | ssim_tauR
+      itr_src itr_tgt
+      (SIM : _ssim ssim RR p_src m_src true m_tgt itr_src itr_tgt)
+    : _ssim ssim RR p_src m_src p_tgt m_tgt itr_src (Tau itr_tgt)
+
+  | ssim_exe
+      tid ktr_src ktr_tgt
+      (SIM : forall rt,
+          ssim _ _ _ RR true m_src true m_tgt (ktr_src rt) (ktr_tgt rt))
+    : _ssim ssim RR p_src m_src p_tgt m_tgt (Vis (inl1 (Execute _ tid)) ktr_src) (Vis (inl1 (Execute _ tid)) ktr_tgt)
+
+  | ssim_obs
+      ktr_src ktr_tgt fn args
+      (SIM : forall r,
+          ssim _ _ _ RR true m_src true m_tgt (ktr_src r) (ktr_tgt r))
+    : _ssim ssim RR p_src m_src p_tgt m_tgt (Vis (inr1 (Observe fn args)) ktr_src) (Vis (inr1 (Observe fn args)) ktr_tgt)
+
+  | ssim_chooseL
+      X ktr_src itr_tgt
+      (SIM : exists x, _ssim ssim RR true m_src p_tgt m_tgt (ktr_src x) itr_tgt)
+    : _ssim ssim RR p_src m_src p_tgt m_tgt (Vis (inr1 (Choose X)) ktr_src) itr_tgt
+
+  | ssim_chooseR
+      X itr_src ktr_tgt
+      (SIM : forall x, _ssim ssim RR p_src m_src true m_tgt itr_src (ktr_tgt x))
+    : _ssim ssim RR p_src m_src p_tgt m_tgt itr_src (Vis (inr1 (Choose X)) ktr_tgt)
+
+  | ssim_fairL
+      f_src ktr_src itr_tgt
+      (SIM : exists m_src0, (<<FAIR : fair_update m_src m_src0 f_src>>) /\
+                         (<<SIM : _ssim ssim RR true m_src0 p_tgt m_tgt (ktr_src tt) itr_tgt>>))
+    : _ssim ssim RR p_src m_src p_tgt m_tgt (Vis (inr1 (Fair f_src)) ktr_src) itr_tgt
+
+  | ssim_fairR
+      f_tgt itr_src ktr_tgt
+      (SIM : forall m_tgt0 (FAIR : fair_update m_tgt m_tgt0 f_tgt),
+          _ssim ssim RR p_src m_src true m_tgt0 itr_src (ktr_tgt tt))
+    : _ssim ssim RR p_src m_src p_tgt m_tgt itr_src (Vis (inr1 (Fair f_tgt)) ktr_tgt)
+
+  | ssim_ub
+      ktr_src itr_tgt
+    : _ssim ssim RR p_src m_src p_tgt m_tgt (Vis (inr1 Undefined) ktr_src) itr_tgt
+
+  | ssim_progress
+      itr_src itr_tgt
+      (PSRC : p_src = true) (PTGT : p_tgt = true)
+      (SIM : ssim _ _ _ RR false m_src false m_tgt itr_src itr_tgt)
+    : _ssim ssim RR p_src m_src p_tgt m_tgt itr_src itr_tgt
+  .
+
+  Definition ssim : forall RT R0 R1 (RR : R0 -> R1 -> Prop), bool -> (@imap thread_id wf_src) -> bool -> (@imap thread_id wf_tgt) -> scheduler RT R0 -> scheduler RT R1 -> Prop
+    := paco10 _ssim bot10.
+
+  Fixpoint ssim_ind
+    (ssim : forall RT R0 R1 (RR : R0 -> R1 -> Prop), bool -> imap wf_src -> bool -> imap wf_tgt -> scheduler RT R0 -> scheduler RT R1 -> Prop)
+    (RT R0 R1 : Type) (RR : R0 -> R1 -> Prop)
+    (P : bool -> @imap thread_id wf_src -> bool -> @imap thread_id wf_tgt -> scheduler RT R0 -> scheduler RT R1 -> Prop)
+    (RET : forall (p_src : bool) (m_src : imap wf_src) (p_tgt : bool) (m_tgt : imap wf_tgt) (r_src : R0) (r_tgt : R1),
+        RR r_src r_tgt -> P p_src m_src p_tgt m_tgt (Ret r_src) (Ret r_tgt))
+    (TAUL : forall (p_src : bool) (m_src : imap wf_src) (p_tgt : bool) (m_tgt : imap wf_tgt) (itr_src : scheduler RT R0) (itr_tgt : scheduler RT R1),
+        _ssim ssim RR true m_src p_tgt m_tgt itr_src itr_tgt ->
+        P true m_src p_tgt m_tgt itr_src itr_tgt -> P p_src m_src p_tgt m_tgt (Tau itr_src) itr_tgt)
+    (TAUR : forall (p_src : bool) (m_src : imap wf_src) (p_tgt : bool) (m_tgt : imap wf_tgt) (itr_src : scheduler RT R0)
+              (itr_tgt : scheduler RT R1),
+        _ssim ssim RR p_src m_src true m_tgt itr_src itr_tgt ->
+        P p_src m_src true m_tgt itr_src itr_tgt -> P p_src m_src p_tgt m_tgt itr_src (Tau itr_tgt))
+    (EXE : forall (p_src : bool) (m_src : imap wf_src) (p_tgt : bool) (m_tgt : imap wf_tgt) (tid : id)
+             (ktr_src : option RT -> scheduler RT R0) (ktr_tgt : option RT -> scheduler RT R1),
+        (forall rt : option RT, ssim RT R0 R1 RR true m_src true m_tgt (ktr_src rt) (ktr_tgt rt)) ->
+        P p_src m_src p_tgt m_tgt (Vis (Execute RT tid|)%sum ktr_src) (Vis (Execute RT tid|)%sum ktr_tgt))
+    (OBS : forall (p_src : bool) (m_src : imap wf_src) (p_tgt : bool) (m_tgt : imap wf_tgt)
+             (ktr_src : nat -> scheduler RT R0) (ktr_tgt : nat -> scheduler RT R1) (fn : nat) (args : list nat),
+        (forall r : nat, ssim RT R0 R1 RR true m_src true m_tgt (ktr_src r) (ktr_tgt r)) ->
+        P p_src m_src p_tgt m_tgt (Vis (|Observe fn args)%sum ktr_src) (Vis (|Observe fn args)%sum ktr_tgt))
+    (CHOOSEL : forall (p_src : bool) (m_src : imap wf_src) (p_tgt : bool) (m_tgt : imap wf_tgt) (X : Type)
+                 (ktr_src : X -> scheduler RT R0) (itr_tgt : scheduler RT R1),
+        (exists x : X, _ssim ssim RR true m_src p_tgt m_tgt (ktr_src x) itr_tgt /\
+                    P true m_src p_tgt m_tgt (ktr_src x) itr_tgt) ->
+        P p_src m_src p_tgt m_tgt (Vis (|Choose X)%sum ktr_src) itr_tgt)
+    (CHOOSER : forall (p_src : bool) (m_src : imap wf_src) (p_tgt : bool) (m_tgt : imap wf_tgt) (X : Type)
+                 (itr_src : scheduler RT R0) (ktr_tgt : X -> scheduler RT R1),
+        (forall x : X, _ssim ssim RR p_src m_src true m_tgt itr_src (ktr_tgt x)) ->
+        (forall x : X, P p_src m_src true m_tgt itr_src (ktr_tgt x)) ->
+        P p_src m_src p_tgt m_tgt itr_src (Vis (|Choose X)%sum ktr_tgt))
+    (FAIRL : forall (p_src : bool) (m_src : imap wf_src) (p_tgt : bool) (m_tgt : imap wf_tgt) (f_src : fmap)
+               (ktr_src : () -> scheduler RT R0) (itr_tgt : scheduler RT R1),
+        (exists m_src0 : imap wf_src,
+            (<< FAIR : fair_update m_src m_src0 f_src >>) /\
+              (<< SIM : _ssim ssim RR true m_src0 p_tgt m_tgt (ktr_src ()) itr_tgt >>) /\
+              P true m_src0 p_tgt m_tgt (ktr_src ()) itr_tgt) ->
+        P p_src m_src p_tgt m_tgt (Vis (|Fair f_src)%sum ktr_src) itr_tgt)
+    (FAIRR : forall (p_src : bool) (m_src : imap wf_src) (p_tgt : bool) (m_tgt : imap wf_tgt) (f_tgt : fmap)
+               (itr_src : scheduler RT R0) (ktr_tgt : () -> scheduler RT R1),
+        (forall m_tgt0 : imap wf_tgt,
+            fair_update m_tgt m_tgt0 f_tgt -> _ssim ssim RR p_src m_src true m_tgt0 itr_src (ktr_tgt ())) ->
+        (forall m_tgt0 : imap wf_tgt, fair_update m_tgt m_tgt0 f_tgt -> P p_src m_src true m_tgt0 itr_src (ktr_tgt ())) ->
+        P p_src m_src p_tgt m_tgt itr_src (Vis (|Fair f_tgt)%sum ktr_tgt))
+    (UB : forall (p_src : bool) (m_src : imap wf_src) (p_tgt : bool) (m_tgt : imap wf_tgt)
+            (ktr_src : void -> itree (schedulerE RT +' eventE) R0) (itr_tgt : scheduler RT R1),
+        P p_src m_src p_tgt m_tgt (Vis (|Undefined)%sum ktr_src) itr_tgt)
+    (PROGRESS : forall (p_src : bool) (m_src : imap wf_src) (p_tgt : bool) (m_tgt : imap wf_tgt) (itr_src : scheduler RT R0)
+                  (itr_tgt : scheduler RT R1),
+        p_src = true ->
+        p_tgt = true ->
+        ssim RT R0 R1 RR false m_src false m_tgt itr_src itr_tgt -> P p_src m_src p_tgt m_tgt itr_src itr_tgt)
+    p_src m_src p_tgt m_tgt (sch_src : scheduler RT R0) (sch_tgt : scheduler RT R1)
+    (SIM : _ssim ssim RR p_src m_src p_tgt m_tgt sch_src sch_tgt) : P p_src m_src p_tgt m_tgt sch_src sch_tgt.
+  Proof.
+    inv SIM; eauto.
+    - eapply TAUL. eauto. eapply ssim_ind; eauto.
+    - eapply TAUR. eauto. eapply ssim_ind; eauto.
+    - eapply CHOOSEL. des. esplits. eauto. eapply ssim_ind; eauto.
+    - eapply CHOOSER. eauto. i. eapply ssim_ind; eauto.
+    - eapply FAIRL. des. esplits; eauto. eapply ssim_ind; eauto.
+    - eapply FAIRR. eauto. i. eapply ssim_ind; eauto.
+  Qed.
+
+  Lemma ssim_mon : monotone10 _ssim.
+  Proof. ii. induction IN using ssim_ind; des; econs; eauto. Qed.
+
+  Hint Constructors _ssim : core.
+  Hint Unfold ssim : core.
+  Hint Resolve ssim_mon : paco.
+  Hint Resolve cpn10_wcompat : paco.
+
+  Lemma ssim_deflag RT R0 R1 (RR : R0 -> R1 -> Prop)
+    p_src p_tgt p_src' p_tgt'
+    m_src m_tgt (sched_src : scheduler RT R0) sched_tgt :
+    ssim RR p_src m_src p_tgt m_tgt sched_src sched_tgt ->
+    ssim RR p_src' m_src p_tgt' m_tgt sched_src sched_tgt.
+  Proof.
+    i. revert p_src' p_tgt'. punfold H.
+    induction H using ssim_ind; i.
+    - pfold. econs; eauto.
+    - pfold. econs. specialize (IH_ssim true p_tgt'). punfold IH_ssim.
+    - pfold. econs. specialize (IH_ssim p_src' true). punfold IH_ssim.
+    - pfold. econs; eauto.
+    - pfold. econs; eauto.
+    - pfold. econs. des. eexists. specialize (H0 true p_tgt'). punfold H0.
+    - pfold. econs. i. specialize (H0 x p_src' true). punfold H0.
+    - pfold. econs. des. esplits; eauto. specialize (H1 true p_tgt'). punfold H1.
+    - pfold. econs. i. specialize (H0 m_tgt0 FAIR p_src' true). punfold H0.
+    - pfold. econs.
+    - clarify. pclearbot.
+      
+      revert p_src' p_tgt' itr_src itr_tgt m_src m_tgt H1.
+      pcofix CIH. i.
+      
+      remember false as p_src0 in H1 at 1.
+      remember false as p_tgt0 in H1 at 1.
+      assert (P_SRC : p_src0 = true -> p_src' = true) by (subst; ss).
+      assert (P_TGT : p_tgt0 = true -> p_tgt' = true) by (subst; ss).
+      clear Heqp_src0 Heqp_tgt0.
+      revert p_src' p_tgt' P_SRC P_TGT. punfold H1.
+      induction H1 using ssim_ind; i.
+      + pfold. econs; eauto.
+      + pfold. econs. specialize (IH_ssim true p_tgt' ltac:(ss) P_TGT). punfold IH_ssim.
+      + pfold. econs. specialize (IH_ssim p_src' true P_SRC ltac:(ss)). punfold IH_ssim.
+      + pfold. econs; eauto. i. eapply upaco10_mon; ss.
+      + pfold. econs; eauto. i. eapply upaco10_mon; ss.
+      + pfold. econs. des. eexists. specialize (H0 true p_tgt' ltac:(ss) P_TGT). punfold H0.
+      + pfold. econs. i. specialize (H0 x p_src' true P_SRC ltac:(ss)). punfold H0.
+      + pfold. econs. des. esplits; eauto. specialize (H1 true p_tgt' ltac:(ss) P_TGT). punfold H1.
+      + pfold. econs. i. specialize (H0 m_tgt0 FAIR p_src' true P_SRC ltac:(ss)). punfold H0.
+      + pfold. econs.
+      + pfold. econs; eauto. pclearbot. right. eapply CIH; eauto.
+  Qed.
+
+End SSIM.
+
+#[export] Hint Constructors _ssim : core.
+#[export] Hint Unfold ssim : core.
+#[export] Hint Resolve ssim_mon : paco.
+
 Section SIM.
 
   Context {_Ident : ID}.
@@ -42,280 +227,13 @@ Section SIM.
   Let eventE1 := @eventE _Ident.
   Let eventE2 := @eventE (sum_tid _Ident).
 
-  Variable wf : WF.
   Variable State : Type.
-  Variable R : Type.
 
   Let thread R := thread _Ident (sE State) R.
   Import Th.
 
-  Lemma Empty_nil s : IdSet.Empty s -> IdSet.elements s = [].
-  Proof.
-    i. destruct s as [s OK]; ss. destruct s; ss.
-    exfalso. eapply H. econs. ss.
-  Qed.
-
-  Lemma Empty_nil_neg s : ~ IdSet.Empty s -> IdSet.elements s <> [].
-  Proof.
-    destruct s as [s SORTED]; ss.
-    ii. subst. eapply H. ii. eapply InA_nil; eauto.
-  Qed.
-
-  Lemma In_MapsTo A k e (m : Th.t A) : List.In (k, e) (elements m) -> MapsTo k e m.
-  Proof.
-    unfold MapsTo, Raw.PX.MapsTo, elements, Raw.elements.
-    remember (this m) as l. clear m Heql. intros.
-    induction l; ss. destruct H.
-    - eapply InA_cons_hd. subst. ss.
-    - eapply InA_cons_tl. eauto.
-  Qed.
-
-  Lemma In_th_proj1 A k (m : Th.t A) : List.In k (th_proj1 m) -> exists e, MapsTo k e m.
-  Proof.
-    unfold th_proj1, MapsTo, Raw.PX.MapsTo, elements, Raw.elements.
-    remember (this m) as l. clear m Heql. intros.
-    induction l; ss. destruct H.
-    - eexists. eapply InA_cons_hd. subst. ss.
-    - eapply IHl in H. destruct H. eexists. eapply InA_cons_tl. eauto.
-  Qed.
-
-  Lemma IdSet_Permutation_remove x s l :
-    Permutation (IdSet.elements s) (x :: l) -> Permutation (IdSet.elements (IdSet.remove x s)) l.
-  Proof.
-    destruct s as [s SORTED]. ss.
-    revert l. induction s; i.
-    - eapply Permutation_length in H. ss.
-    - assert (List.In a (x :: l)) by (rewrite <- H; econs; ss).
-      destruct H0.
-      + subst. eapply Permutation_cons_inv in H. ss.
-        Raw.MX.elim_comp_eq a a. ss.
-      + eapply Add_inv in H0. des. eapply Permutation_Add in H0.
-        rewrite <- H0 in *. clear l H0.
-        rewrite perm_swap in H. eapply Permutation_cons_inv in H.
-        assert (List.In x s).
-        { eapply Permutation_in.
-          - symmetry. eapply H.
-          - econs; ss.
-        }
-        eapply IdSet.MSet.Raw.isok_iff in SORTED.
-        epose proof (Sorted_extends _ SORTED).
-        eapply Forall_forall in H1; eauto.
-        ss. Raw.MX.elim_comp_gt x a.
-        econs. eapply IHs; eauto.
-        eapply IdSet.MSet.Raw.isok_iff.
-        inv SORTED; ss.
-    Unshelve. compute. lia.
-  Qed.
-
-  Lemma IdSet_Permutation_add x s l :
-    ~ IdSet.In x s -> Permutation (IdSet.elements s) l -> Permutation (IdSet.elements (IdSet.add x s)) (x :: l).
-  Proof.
-    destruct s as [s SORTED]. ss. revert l. induction s; intros l H1 H2.
-    - rewrite <- H2. ss.
-    - ss. assert (x = a \/ x < a \/ x > a) by lia. des.
-      + exfalso. eapply H1. econs. ss.
-      + Raw.MX.elim_comp_lt x a. econs. ss.
-      + Raw.MX.elim_comp_gt x a. rewrite <- H2. rewrite perm_swap. econs.
-        eapply IHs; eauto.
-        unfold IdSet.In, IdSet.MSet.In in *. ss.
-        intro. eapply H1. econs 2. eapply H0.
-        Unshelve. clear H1. eapply IdSet.MSet.Raw.isok_iff in SORTED. inv SORTED.
-        eapply IdSet.MSet.Raw.isok_iff. ss.
-  Qed.
-
-  Lemma Permutation_remove A k e (m : Th.t A) l :
-    Permutation (elements m) ((k, e) :: l) -> Permutation (elements (remove k m)) l.
-  Proof.
-    unfold elements, Raw.elements, remove.
-    destruct m as [m SORTED]. ss.
-    revert l. induction m; i.
-    - eapply Permutation_length in H. ss.
-    - assert (List.In a ((k, e) :: l)) by (rewrite <- H; econs; ss).
-      destruct H0.
-      + inv H0. eapply Permutation_cons_inv in H. ss.
-        Raw.MX.elim_comp_eq k k. eauto.
-    + eapply Add_inv in H0. destruct H0. eapply Permutation_Add in H0.
-      rewrite <- H0 in *. clear l H0.
-      rewrite perm_swap in H. eapply Permutation_cons_inv in H.
-      assert (List.In (k, e) m).
-      { eapply Permutation_in.
-        - symmetry; eauto.
-        - econs; ss.
-      }
-      epose proof (Sorted_extends _ SORTED).
-      eapply Forall_forall in H1; eauto.
-      destruct a. ss. Raw.MX.elim_comp_gt k n.
-      inv SORTED.
-      econs. eapply IHm; eauto.
-    Unshelve. compute. lia.
-  Qed.
-
-  Lemma Permutation_add A k e (m : Th.t A) l :
-    ~ In k m -> Permutation (elements m) l -> Permutation (elements (add k e m)) ((k, e) :: l).
-  Proof.
-    unfold elements, Raw.elements, add, In.
-    destruct m as [m SORTED]. ss. revert l. induction m; intros l H1 H2.
-    - rewrite <- H2. ss.
-    - destruct a. ss.
-      assert (k = n \/ k < n \/ k > n) by lia.
-      destruct H as [|[]].
-      + exfalso. eapply H1. exists a. left. ss.
-      + Raw.MX.elim_comp_lt k n. econs; eauto.
-      + Raw.MX.elim_comp_gt k n.
-        rewrite <- H2. rewrite perm_swap. econs.
-        inv SORTED. eapply IHm; eauto.
-        intro. eapply H1. unfold Raw.PX.In in *.
-        destruct H0. eexists. right. eauto.
-  Qed.
-
-  Lemma InA_In A x (l : list A) : InA (@eq A) x l -> List.In x l.
-  Proof. i. induction H.
-         - left; eauto.
-         - right; eauto.
-  Qed.
-    
-  Lemma setoid_in_in A k (e : A) l :
-    SetoidList.InA (@eq_key_elt A) (k, e) l -> List.In (k, e) l.
-  Proof.
-    i. induction H.
-    - left. destruct H; ss. subst. destruct y; ss.
-    - right. eauto.
-  Qed.
-
-  Lemma Permutation_NoDupA A l1 l2 :
-    Permutation l1 l2 ->
-    SetoidList.NoDupA (eq_key (elt:=A)) l1 ->
-    SetoidList.NoDupA (eq_key (elt:=A)) l2.
-  Proof.
-    i.
-    eapply PermutationA_preserves_NoDupA; eauto.
-    eapply Permutation_PermutationA; eauto.
-  Qed.
-
   Lemma nth_error_Some' A (l : list A) x i : nth_error l i = Some x -> i < List.length l.
   Proof. i. eapply nth_error_Some. intro. rewrite H in H0; ss. Qed.
-
-  Theorem ssim_nondet_fifo
-    p_src p_tgt tid ths_src ths_tgt
-    (THREADS : Permutation (IdSet.elements ths_src) ths_tgt)
-    (TID : ~ IdSet.In tid ths_src)
-    : forall m_tgt, exists m_src, @ssim nat_wf nat_wf R R R eq p_src m_src p_tgt m_tgt
-                          (schedule_nondet R (tid, ths_src))
-                          (schedule_fifo R (tid, ths_tgt)).
-  Proof.
-    i.
-
-    remember (fun (i : thread_id.(id)) => List.length ths_tgt + 1) as m_src.
-    assert (M_SRC0 : m_src tid > List.length ths_tgt) by (subst; lia).
-    assert (M_SRC1 : forall i tid, nth_error ths_tgt i = Some tid -> m_src tid > i).
-    { subst. i. eapply nth_error_Some' in H. lia. }
-    clear Heqm_src.
-    exists m_src.
-
-    revert p_src p_tgt m_src m_tgt tid ths_src ths_tgt THREADS TID M_SRC0 M_SRC1.
-    pcofix CIH. i.
-
-    rewrite unfold_schedule_nondet.
-    rewrite unfold_schedule_fifo.
-    rewrite ! bind_trigger.
-    pfold. econs. intros [].
-    - left.
-      destruct (IdSet.is_empty ths_src) eqn: H.
-      + eapply IdSet.is_empty_2 in H.
-        eapply Empty_nil in H.
-        rewrite H in THREADS.
-        eapply Permutation_nil in THREADS.
-        subst ths_tgt.
-        pfold. econs; ss.
-      + assert (~ IdSet.Empty ths_src).
-        { ii. eapply IdSet.is_empty_1 in H0. rewrite H in H0; ss. }
-        clear H. eapply Empty_nil_neg in H0.
-        destruct ths_tgt as [| tid' ths_tgt' ].
-        { symmetry in THREADS. eapply Permutation_nil in THREADS. ss. }
-        pfold. eapply ssim_chooseL. exists tid'. unfold id_pop.
-        replace (IdSet.mem tid' ths_src) with true; cycle 1.
-        { symmetry. eapply IdSet.mem_1. eapply In_InA; eauto.
-          rewrite THREADS. econs; ss.
-        }
-        rewrite bind_trigger.
-        eapply ssim_fairL.
-        remember (fun i => if Nat.eqb i tid'
-                        then List.length ths_tgt' + 1
-                        else m_src i - 1) as m_src'.
-        exists m_src'. splits.
-        { ii. unfold tids_fmap. des_if; ss. subst.
-          replace (i =? tid')%nat with false by (symmetry; eapply Nat.eqb_neq; eauto).
-          des_if.
-          - assert (List.In i (IdSet.elements ths_src)).
-            { eapply InA_In. eapply IdSet.remove_3. eapply In_InA; eauto. eapply i0. }
-            rewrite THREADS in H.
-            eapply In_nth_error in H. destruct H as [i' H].
-            enough (m_src i > i') by lia.
-            eapply M_SRC1; eauto.
-          - unfold le; ss. lia.
-        }
-        do 3 econs; eauto. right. eapply CIH.
-        * eapply IdSet_Permutation_remove. eapply THREADS.
-        * eapply IdSet.remove_1; ss.
-        * subst. replace (tid' =? tid')%nat with true by (symmetry; eapply Nat.eqb_refl). lia.
-        * subst. i. des_if.
-          -- eapply nth_error_Some' in H. lia.
-          -- enough (m_src tid0 > 1 + i) by lia. eapply M_SRC1. eauto.
-    - left.
-      match goal with
-      | [ |- paco10 _ _ _ _ _ _ _ _ _ _ _ (match ?x with
-                                          | [] => _
-                                          | t' :: ts' => _
-                                          end)] => destruct x as [| tid' ths_tgt'] eqn: E_ths_tgt
-      end.
-      { eapply app_eq_nil in E_ths_tgt. des. ss. }
-      pfold. eapply ssim_chooseL. exists tid'. unfold id_pop.
-      replace (IdSet.mem tid' (IdSet.add tid ths_src)) with true; cycle 1.
-      { symmetry. eapply IdSet.mem_1.
-        destruct ths_tgt; ss; inversion E_ths_tgt; subst.
-        - eapply IdSet.add_1; ss.
-        - eapply IdSet.add_2. eapply In_InA; eauto. rewrite THREADS. econs; ss.
-      }
-      rewrite bind_trigger. eapply ssim_fairL.
-      remember (fun i => if Nat.eqb i tid'
-                      then List.length ths_tgt' + 1
-                      else m_src i - 1) as m_src'.
-      exists m_src'. splits.
-      { ii. unfold tids_fmap. des_if; ss. subst.
-        replace (i =? tid')%nat with false by (symmetry; eapply Nat.eqb_neq; eauto).
-        des_if.
-        - assert (List.In i (IdSet.elements (IdSet.add tid ths_src))).
-          { eapply InA_In. eapply IdSet.remove_3. eapply In_InA; eauto. eapply i0. }
-          assert (i = tid \/ i <> tid) by lia.
-          destruct H0.
-          + subst. lia.
-          + assert (List.In i (IdSet.elements ths_src)).
-            { eapply InA_In. eapply IdSet.add_3; eauto. eapply In_InA; eauto. }
-            rewrite THREADS in H1. eapply In_nth_error in H1. destruct H1 as [i' H1].
-            enough (m_src i > i') by lia.
-            eapply M_SRC1; eauto.
-        - unfold le; ss. lia.
-      }
-      do 3 econs; ss. right. unfold IdSet.elt in *. eapply CIH.
-      + eapply IdSet_Permutation_remove.
-        rewrite IdSet_Permutation_add.
-        * eapply Permutation_refl' in E_ths_tgt. rewrite Permutation_app_comm in E_ths_tgt. eapply E_ths_tgt.
-        * intro H. eapply TID. eapply H.
-        * ss.
-      + eapply IdSet.remove_1; ss.
-      + subst. replace (tid' =? tid')%nat with true by (symmetry; eapply Nat.eqb_refl). lia.
-      + subst. i. des_if.
-        * eapply nth_error_Some' in H. lia.
-        * enough (m_src tid0 > 1 + i) by lia.
-          assert (nth_error (ths_tgt ++ [tid]) (1 + i) = Some tid0) by (rewrite E_ths_tgt; ss).
-          assert (1 + i < List.length ths_tgt \/ 1 + i >= List.length ths_tgt) by lia.
-          destruct H1.
-          -- rewrite nth_error_app1 in H0 by ss. eapply M_SRC1; eauto.
-          -- rewrite nth_error_app2 in H0 by ss.
-             assert (1 + i - List.length ths_tgt = 0)
-               by (destruct (1 + i - List.length ths_tgt) as [|[]] in *; ss).
-             rewrite H2 in H0. inversion H0. subst. lia.
-  Qed.
 
   Theorem ssim_implies_gsim
     RT R0 R1 RR p_src p_tgt sched_src sched_tgt
@@ -336,7 +254,7 @@ Section SIM.
                 | inr i => gm_tgt (inr i)
                 end) as gm_src.
     assert (M_SRC0 : forall i, gm_src (inl i) = m_src i) by (subst; ss).
-    assert (M_SRC1 : forall i, nat_wf.(le) (gm_tgt (inr i)) (gm_src (inr i))) by (subst; reflexivity).
+    assert (M_SRC1 : forall i, le nat_wf (gm_tgt (inr i)) (gm_src (inr i))) by (subst; reflexivity).
     clear Heqm_tgt Heqgm_src.
     exists gm_src.
  
@@ -434,31 +352,5 @@ Section SIM.
       gstep. eapply sim_ub.
     - gstep. econs; eauto. pclearbot. gfinal. left. eapply CIH; eauto.
   Qed.
-
-  Check ssim_nondet_fifo.
-  Check ssim_implies_gsim.
-
-  Definition key_set {elt} : Th.t elt -> IdSet.t.
-  Proof.
-    intros [l SORTED]. unfold Raw.t in *.
-    set (l' := List.map fst l).
-    econs. instantiate (1 := l').
-    unfold Raw.PX.ltk in *.
-
-    assert (Sorted (fun x y => x < y) l').
-    { induction SORTED.
-      - subst l'. ss.
-      - subst l'. ss. econs 2; ss.
-        inv H; ss. econs; ss.
-    }
-    
-    eapply IdSet.MSet.Raw.isok_iff. ss.
-  Defined.
-
-  Theorem sched_sim p_src p_tgt tid st (ths : @threads _Ident (sE State) R) (TID : ~ IdSet.In tid (key_set ths))
-    : gsim nat_wf nat_wf eq p_src p_tgt
-        (interp_state (st, interp_sched (ths, schedule_nondet _ (tid, key_set ths))))
-        (interp_state (st, interp_sched (ths, schedule_fifo _ (tid, IdSet.elements (key_set ths))))).
-  Proof. eapply ssim_implies_gsim. eapply ssim_nondet_fifo; ss. Qed.
 
 End SIM.
